direction derives => reaches for PDA M

autth/CFG_to_PDA.lean
@@ -1,4 +1,5 @@
 import autth.PDA
+import autth.leftmost_deriv
 import Mathlib.Computability.ContextFreeGrammar
 import Mathlib.Logic.Relation
 /-!
@@ -16,26 +17,35 @@ namespace CFG_to_PDA
 open ContextFreeGrammar
 open Symbol
 open PDA
+open ContextFreeRule.RewritesLeftmost
 
 -- In this whole section G will be the grammar we want to convert to a pda
-variable {T : Type} [DecidableEq T] (G : ContextFreeGrammar T)
-
+variable {T : Type} [DecidableEq T][Fintype T]
 structure Q where loop ::
-abbrev S := Symbol T G.NT
-abbrev PDA' := PDA Q T (S G)
 
-abbrev transition_fun (_ : Q) (a : T) (Z : S G) : Set (Q × List (S G)) :=
+instance : Fintype Q where
+  elems := {Q.loop}
+  complete := by intro q; simp
+
+
+abbrev S (G : ContextFreeGrammar T)[Fintype G.NT] := Symbol T G.NT
+
+abbrev PDA' (G : ContextFreeGrammar T)[Fintype G.NT] := PDA Q T (S G)
+
+
+
+abbrev transition_fun (G : ContextFreeGrammar T)[Fintype G.NT] (_ : Q) (a : T) (Z : S G) : Set (Q × List (S G)) :=
   match Z with
   | terminal b => if a=b then {(Q.loop, [])} else {}
   | _ => ∅
 
-abbrev transition_fun' (_ : Q) (Z : S G) : Set (Q × List (S G)) :=
+abbrev transition_fun' (G : ContextFreeGrammar T)[Fintype G.NT] (_ : Q) (Z : S G) : Set (Q × List (S G)) :=
   match Z with
   | nonterminal N => { (Q.loop, α) | (α : List (S G)) (_ : ⟨N, α⟩ ∈ G.rules) }
   | _ => ∅
 
 -- Martin: This is not a good name for a function.
-abbrev M : PDA' G := {
+abbrev M (G : ContextFreeGrammar T)[Fintype G.NT] : PDA' G:= {
   initial_state := Q.loop
   start_symbol := nonterminal G.initial
   final_states := ∅
@@ -43,6 +53,8 @@ abbrev M : PDA' G := {
   transition_fun' := transition_fun' G
 }
 
+section
+variable {G : ContextFreeGrammar T}[Fintype G.NT]
 theorem M_consumes_terminal (a : T) (w : List T) (α : List (S G)):
     (M G).reachesN 1 ⟨Q.loop, a::w, terminal a :: α⟩ ⟨Q.loop, w, α⟩ := by
   rw [reachesN_one,step]
@@ -51,33 +63,154 @@ theorem M_consumes_terminal (a : T) (w : List T) (α : List (S G)):
   use Q.loop, []
   simp [M, CFG_to_PDA.transition_fun]
 
+theorem M_consumes_nonterminal {r : ContextFreeRule T G.NT}(h : r ∈ G.rules)(w : List T) (α : List (S G)):
+    (M G).reachesN 1 ⟨Q.loop, w, nonterminal r.input :: α⟩ ⟨Q.loop, w, r.output ++ α⟩ := by
+  rw [reachesN_one]
+  rcases w with _| ⟨a, w'⟩ <;> dsimp [step]
+  · use Q.loop, r.output
+    dsimp [transition_fun']
+    refine ⟨?_,?_⟩
+    · use r.output
+    · rfl
+  · rw [Set.mem_union]
+    right
+    use Q.loop, r.output
+    dsimp [transition_fun']
+    refine ⟨?_,?_⟩
+    · use r.output
+    · rfl
+
+theorem M_consumes_terminal_string  (w w': List T) (α : List (S G)):
+    (M G).reaches ⟨Q.loop, w++w', w.map terminal ++ α⟩ ⟨Q.loop, w', α⟩ := by
+  induction' w with a w ih
+  · rfl
+  · apply reaches_trans _ ih
+    rw [reaches_iff_reachesN]
+    use 1
+    apply M_consumes_terminal
+
+theorem M_terminal_stack_of_read (a : T) (w : List T) (α β : List (S G)):
+    (M G).reachesN 1 ⟨Q.loop, a::w, α⟩ ⟨Q.loop, w, β ⟩ → α = terminal a::β  := by
+  intro h
+  rcases α with _|⟨Z,α'⟩ <;> rw [reachesN_one] at h <;> dsimp [step] at h
+  · rw [Set.mem_singleton_iff] at h
+    have : w = a::w := by apply conf.mk.inj at h; exact h.2.1
+    apply List.ne_cons_self at this
+    contradiction
+  · rw [Set.mem_union] at h
+    rcases h with h|h
+    <;> rw [Set.mem_setOf] at h
+    <;> obtain ⟨_,γ,hγ, hr⟩ := h
+    <;> rcases Z with ⟨a₀⟩|⟨N⟩
+    <;> dsimp [transition_fun,transition_fun'] at hγ
+    · have : a=a₀ ∨ a≠a₀ := by exact Decidable.em (a=a₀)
+      rcases this with h|h <;> simp [h] at hγ
+      · apply conf.mk.inj at hr
+        simp [hr,h,hγ]
+    · rw [Set.mem_empty_iff_false] at hγ
+      contradiction
+    · rw [Set.mem_empty_iff_false] at hγ
+      contradiction
+    · rw [conf.mk.injEq] at hr
+      exfalso
+      exact List.cons_ne_self _ _ hr.2.1.symm
+
+
+theorem M_deterministic_step_of_terminal_stack_cons (a: T)(w v: List T) (β β': List (S G)):
+    (M G).reachesN 1 ⟨Q.loop, w, terminal a :: β⟩ ⟨Q.loop, v, β'⟩ → w=a::v ∧ β = β' := by
+  intro h
+  rw [reachesN_one] at h
+  rcases w with _|⟨b, w'⟩ <;>  dsimp [step, transition_fun'] at h
+  · obtain ⟨_,β',h⟩ := h
+    exfalso
+    exact (Set.mem_empty_iff_false _).mp h.1
+  · rw [Set.mem_union, Set.mem_setOf,Set.mem_setOf] at h
+    rcases h with ⟨_,γ,hγ, h⟩|⟨_,γ ,hγ, h⟩
+    · rcases dec_em (a = b) with h'|h'<;> simp only [transition_fun, Set.mem_ite_empty_right] at hγ
+      · apply conf.mk.inj at h
+        rw [Set.mem_singleton_iff, Prod.mk.inj_iff] at hγ
+        rw [h.2.1,hγ.1,h',h.2.2,hγ.2.2]
+        simp
+      · exfalso
+        exact h' hγ.1.symm
+    · exfalso
+      exact (Set.not_mem_empty _) hγ
+
+theorem M_deterministic_of_terminal_stack_cons (a: T)(w : List T) (β : List (S G)):
+    (M G).reaches ⟨Q.loop, w, terminal a :: β⟩ ⟨Q.loop, [], []⟩ →
+    ∃w' : List T, w = a :: w' ∧ (M G).reaches ⟨Q.loop, w', β⟩ ⟨Q.loop, [], []⟩ := by
+  intro h
+  rw [reaches_iff_reachesN] at h
+  obtain ⟨n,h⟩ := h
+  rcases n with _|⟨n⟩
+  · rw [reachesN_zero,conf.mk.injEq] at h
+    exfalso
+    exact List.cons_ne_nil _ _ h.2.2
+  · rw [←reachesN_iff_split_first] at h
+    obtain ⟨⟨_,v,β'⟩,h₁,h₂⟩ := h
+    apply M_deterministic_step_of_terminal_stack_cons at h₁
+    use v
+    use h₁.1
+    rw [←h₁.2] at h₂
+    rw [reaches_iff_reachesN]
+    use n
+
+theorem M_deterministic_of_terminal_stack (w v: List T) (β  : List (S G)):
+    (M G).reaches ⟨Q.loop, w, v.map terminal ++ β⟩ ⟨Q.loop, [], []⟩ →
+    ∃w' : List T,  w = v ++ w' ∧ (M G).reaches ⟨Q.loop, w', β⟩ ⟨Q.loop, [], []⟩ := by
+  intro h
+  induction' v with a v' ih generalizing w
+  · use w
+    simp at h
+    simp [h]
+  · rw [List.map_cons] at h
+    apply M_deterministic_of_terminal_stack_cons at h
+    obtain ⟨w₀, hw₀,hr⟩ := h
+    apply ih at hr
+    obtain ⟨w₁, hw₁,hr⟩ := hr
+    use w₁
+    refine ⟨?_,?_⟩
+    · simp [hw₀, hw₁]
+    · exact hr
 
 theorem M_reaches_off_G_derives (α : List (Symbol T G.NT)) (w : List T)
-    (h : G.Derives α (w.map terminal)):
+    (h : G.DerivesLeftmost α (w.map terminal)):
     (M G).reaches ⟨Q.loop, w, α⟩ ⟨Q.loop, [], []⟩ := by
-  generalize def_s : w.map terminal = s at h
   induction' h using Relation.ReflTransGen.head_induction_on with α β hα hβ ih
   case refl =>
-    induction' w with a w' ih generalizing s
+    induction' w with a w' ih
     case nil =>
-      rw [←def_s]
       dsimp [reaches]
       use 0
       simp [stepSetN]
     case cons =>
-      rw [List.map_cons] at def_s
-      have := ih (w'.map terminal) rfl
-      rw [reaches_iff_reachesN] at this
-      obtain ⟨n, hw'⟩ := this
+      rw [List.map_cons]
+      rw [reaches_iff_reachesN] at ih
+      obtain ⟨n, hw'⟩ := ih
       rw [reaches_iff_reachesN]
       use n+1
       rw [←reachesN_iff_split_first]
       use ⟨Q.loop, w', w'.map terminal⟩
       refine ⟨?_,?_⟩
-      · rw [←def_s]
-        apply M_consumes_terminal
+      · apply M_consumes_terminal
       · exact hw'
-  sorry
+  case head =>
+    obtain ⟨r,hrg,hrα⟩ := hα
+    rw [rewrites_leftmost_iff] at hrα
+    obtain ⟨p,q,hα',hβ'⟩ := hrα
+    rw [hβ'] at ih
+    rw [List.append_assoc] at ih
+    apply M_deterministic_of_terminal_stack at ih
+    obtain ⟨w', hw', hr ⟩ := ih
+    have hpart₁ : (M G).reaches ⟨Q.loop, w,α⟩ ⟨Q.loop, w', nonterminal r.input :: q ⟩ := by
+      rw [hα', List.append_assoc, hw']
+      apply M_consumes_terminal_string p  _
+    have hpart₂ : (M G).reaches ⟨Q.loop, w', nonterminal r.input :: q⟩ ⟨Q.loop, w', r.output ++ q⟩ := by
+      rw [reaches_iff_reachesN]
+      use 1
+      exact M_consumes_nonterminal hrg _ q
+    have := reaches_trans hpart₁ hpart₂
+    exact reaches_trans this hr
 
 
 theorem G_derives_of_M_reaches {α : List (Symbol T G.NT)} {w : List T}
@@ -89,5 +222,7 @@ theorem G_derives_iff_M_reaches {α : List (Symbol T G.NT)} {w : List T} :
     G.Derives α (w.map terminal) ↔
     (M G).reaches ⟨Q.loop,w, α⟩ ⟨Q.loop,[], []⟩ := by
   sorry
+end section
 
-theorem pda_of_cfg (L : Language T) : L = G.language → L = (M G).acceptsByEmptyStack := by sorry
+
+theorem pda_of_cfg (G : ContextFreeGrammar T)[Fintype G.NT] : G.language  = (M G).acceptsByEmptyStack := by sorry
